fix addition

code/experimental/rsa/Hacl.Impl.Addition.fst
@@ -9,6 +9,38 @@ open Hacl.Impl.Lib
 
 module Buffer = Spec.Lib.IntBuf
 
+
+val addcarry_u64: 
+    carry:uint64 -> a:uint64 -> b:uint64 -> Tot (tuple2 uint64 uint64)
+[@"c_inline"]    
+let addcarry_u64 carry a b =
+    let t1 = add_mod #U64 a carry in
+    let carry = if (lt_u64 t1 carry) then u64 1 else u64 0 in
+    let res = add_mod #U64 t1 b in
+    let carry = if (lt_u64 res t1) then add #U64 carry (u64 1) else carry in
+    (carry, res)
+  
+val subborrow_u64:
+    carry:uint64 -> a:uint64 -> b:uint64 -> Tot (tuple2 uint64 uint64)
+    [@"c_inline"]
+let subborrow_u64 carry a b =
+    let res = sub_mod #U64 (sub_mod #U64 a b) carry in
+    let carry =
+        if (eq_u64 carry (u64 1)) then
+           (if (le_u64 a b) then u64 1 else u64 0)
+        else
+           (if (lt_u64 a b) then u64 1 else u64 0) in
+    (carry, res)
+
+val bval:
+    #bLen:size_nat -> cbLen:size_t{v cbLen == bLen} ->
+    b:lbignum bLen -> i:size_t -> Stack uint64
+    (requires (fun h -> live h b))
+    (ensures (fun h0 _ h1 -> preserves_live h0 h1 /\ h0 == h1))
+    [@"c_inline"]
+let bval #bLen cbLen b i =
+    if (i <. cbLen) then b.(i) else u64 0
+    
 val bn_sub_:
     #aLen:size_nat -> #bLen:size_nat ->
     caLen:size_t{v caLen == aLen} -> a:lbignum aLen ->
@@ -17,18 +49,13 @@ val bn_sub_:
     res:lbignum aLen -> Stack unit
     (requires (fun h -> live h a /\ live h b /\ live h res))
     (ensures (fun h0 _ h1 -> preserves_live h0 h1 /\ modifies1 res h0 h1))
-    
+    [@"c_inline"]
 let rec bn_sub_ #aLen #bLen caLen a cbLen b i carry res =
     if (i <. caLen) then begin
        let t1 = a.(i) in
-       let t2 = if (i <. cbLen) then b.(i) else u64 0 in
-       let res_i = sub_mod #U64 (sub_mod #U64 t1 t2) carry in
+       let t2 = bval cbLen b i in
+       let (carry, res_i) = subborrow_u64 carry t1 t2 in
        res.(i) <- res_i;
-       let carry =
-           if (eq_u64 carry (u64 1)) then
-              (if (le_u64 t1 t2) then u64 1 else u64 0)
-           else
-              (if (lt_u64 t1 t2) then u64 1 else u64 0) in
        bn_sub_ #aLen #bLen caLen a cbLen b (size_incr i) carry res
     end
 
@@ -42,7 +69,7 @@ val bn_sub:
     res:lbignum aLen -> Stack unit
     (requires (fun h -> live h a /\ live h b /\ live h res))
     (ensures (fun h0 _ h1 -> preserves_live h0 h1 /\ modifies1 res h0 h1))
-
+    [@"c_inline"]
 let bn_sub #aLen #bLen caLen a cbLen b res =
     bn_sub_ #aLen #bLen caLen a cbLen b (size 0) (u64 0) res
 
@@ -54,16 +81,13 @@ val bn_add_:
     res:lbignum aLen -> Stack uint64
     (requires (fun h -> live h a /\ live h b /\ live h res))
     (ensures (fun h0 _ h1 -> preserves_live h0 h1 /\ modifies1 res h0 h1))
-    
+    [@"c_inline"]
 let rec bn_add_ #aLen #bLen caLen a cbLen b i carry res =
     if (i <. caLen) then begin
        let t1 = a.(i) in
-       let t2 = if (i <. cbLen) then b.(i) else u64 0 in
-       let t1 = add_mod #U64 t1 carry in
-       let carry = if (lt_u64 t1 carry) then u64 1 else u64 0 in
-       let res_i = add_mod #U64 t1 t2 in
+       let t2 = bval cbLen b i in
+       let (carry, res_i) = addcarry_u64 carry t1 t2 in
        res.(i) <- res_i;
-       let carry = if (lt_u64 res_i t1) then add #U64 carry (u64 1) else carry in
        bn_add_ #aLen #bLen caLen a cbLen b (size_incr i) carry res end
     else carry
 
@@ -74,7 +98,7 @@ val bn_add:
     res:lbignum aLen -> Stack unit
     (requires (fun h -> live h a /\ live h b /\ live h res))
     (ensures (fun h0 _ h1 -> preserves_live h0 h1 /\ modifies1 res h0 h1))
-
+    [@"c_inline"]
 let bn_add #aLen #bLen caLen a cbLen b res =
     let _ = bn_add_ #aLen #bLen caLen a cbLen b (size 0) (u64 0) res in ()
 
@@ -85,22 +109,19 @@ val bn_add_carry:
     res:lbignum (aLen + 1) -> Stack unit
     (requires (fun h -> live h a /\ live h b /\ live h res))
     (ensures (fun h0 _ h1 -> preserves_live h0 h1 /\ modifies1 res h0 h1))
-    
+    [@"c_inline"]
 let bn_add_carry #aLen #bLen caLen a cbLen b res =
     let res' = Buffer.sub #uint64 #(aLen + 1) #aLen res (size 0) caLen in
     let carry = bn_add_ #aLen #bLen caLen a cbLen b (size 0) (u64 0) res' in
     res.(caLen) <- carry
 
-
 val bn_sub_u64_:
-    #aLen:size_nat ->
-    aaLen:size_t{v aaLen == aLen} ->
-    a:lbignum aLen ->
-    carry:uint64 -> i:size_t ->
+    #aLen:size_nat -> aaLen:size_t{v aaLen == aLen} ->
+    a:lbignum aLen -> carry:uint64 -> i:size_t ->
     res:lbignum aLen -> Stack unit
     (requires (fun h -> live h a /\ live h res))
     (ensures (fun h0 _ h1 -> preserves_live h0 h1 /\ modifies1 res h0 h1))
-    
+    [@"c_inline"]
 let rec bn_sub_u64_ #aLen aaLen a carry i res =
     if (i <. aaLen) then begin
        let t1 = a.(i) in
@@ -118,5 +139,5 @@ val bn_sub_u64:
     res:lbignum aLen -> Stack unit
     (requires (fun h -> live h a /\ live h res))
     (ensures (fun h0 _ h1 -> preserves_live h0 h1 /\ modifies1 res h0 h1))
-    
+    [@"c_inline"]
 let bn_sub_u64 #aLen aaLen a b res = bn_sub_u64_ #aLen aaLen a b (size 0) res
